WIP: beh

src/FairBeh.v
@@ -8,6 +8,45 @@ Require Import Coq.Classes.RelationClasses.
 
 Set Implicit Arguments.
 
+Section OBS.
+
+  Variant event: Type :=
+    | event_syscall (fn: nat) (args: list nat) (retv: nat)
+  .
+
+End OBS.
+
+Module Tr.
+  CoInductive t {R}: Type :=
+  | done (retv: R)
+  | spin
+  | ub
+  | nb
+  | cons (hd: event) (tl: t)
+  .
+  Infix "##" := cons (at level 60, right associativity).
+
+  Fixpoint app {R} (pre: list event) (bh: @t R): t :=
+    match pre with
+    | [] => bh
+    | hd :: tl => cons hd (app tl bh)
+    end
+  .
+
+  Lemma fold_app
+        R s pre tl
+    :
+      (Tr.cons s (Tr.app pre tl)) = @Tr.app R (s :: pre) tl
+  .
+  Proof. reflexivity. Qed.
+
+  Definition prefix {R} (pre: list event) (bh: @t R): Prop :=
+    exists tl, <<PRE: app pre tl = bh>>
+  .
+
+End Tr.
+
+
 Module Flag.
 
   Variant t: Type :=
@@ -36,6 +75,7 @@ Module Flag.
 
 End Flag.
 
+
 Class ID : Type := mk { id: Type }.
 
 Section EVENT.
@@ -44,23 +84,15 @@ Section EVENT.
 
   Variant eventE: Type -> Type :=
     | Choose (X: Type): eventE X
-    | Fair (m: Ident.(id) -> Flag.t): eventE unit
+    | Fair (m: id -> Flag.t): eventE unit
+    | Syscall (fn: nat) (args: list nat) (retv: nat): eventE nat
   .
 
 End EVENT.
 
 
-
-Module Tr.
-  CoInductive t: Type :=
-  | done
-  | spin
-  .
-End Tr.
-
 Section BEHAVES.
 
-  (* Variable Ident: Type. *)
   Context {Ident: ID}.
 
   Inductive terminate
@@ -73,45 +105,56 @@ Section BEHAVES.
     terminate (Ret r)
   | terminate_tau
       itr
-      (DIV: terminate itr)
+      (TERM: terminate itr)
     :
     terminate (Tau itr)
   | terminate_choose
       X ktr x
-      (DIV: terminate (ktr x))
+      (TERM: terminate (ktr x))
     :
     terminate (Vis (Choose X) ktr)
   | terminate_fair
       m ktr
-      (DIV: terminate (ktr tt))
+      (TERM: terminate (ktr tt))
     :
     terminate (Vis (Fair m) ktr)
+  | terminate_syscall
+      fn args retv ktr
+      (TERM: terminate (ktr retv))
+    :
+    terminate (Vis (Syscall fn args retv) ktr)
   .
 
   Variant _diverge_index
-          (diverge_index: forall (R: Type) (idx: Ident.(id) -> nat) (itr: itree eventE R), Prop)
+          (diverge_index: forall (R: Type) (idx: id -> nat) (itr: itree eventE R), Prop)
           (R: Type)
     :
-    forall (idx: Ident.(id) -> nat) (itr: itree eventE R), Prop :=
-  | diverge_index_tau
-      itr idx0 idx1
-      (DIV: diverge_index _ idx1 itr)
-      (IDX: forall i, idx1 i <= idx0 i)
-    :
-    _diverge_index diverge_index idx0 (Tau itr)
-  | diverge_index_choose
-      X ktr x idx0 idx1
-      (DIV: diverge_index _ idx1 (ktr x))
-      (IDX: forall i, idx1 i <= idx0 i)
-    :
-    _diverge_index diverge_index idx0 (Vis (Choose X) ktr)
-  | diverge_index_fair
-      m ktr idx0 idx1
-      (DIV: diverge_index _ idx1 (ktr tt))
-      (EMP: forall j (IDX: (m j) = Flag.emp), idx1 j <= idx0 j)
-      (FAIL: forall j (IDX: (m j) = Flag.fail), idx1 j < idx0 j)
-    :
-    _diverge_index diverge_index idx0 (Vis (Fair m) ktr)
+    forall (idx: id -> nat) (itr: itree eventE R), Prop :=
+    | diverge_index_tau
+        itr idx0 idx1
+        (DIV: diverge_index _ idx1 itr)
+        (IDX: forall i, idx1 i <= idx0 i)
+      :
+      _diverge_index diverge_index idx0 (Tau itr)
+    | diverge_index_choose
+        X ktr x idx0 idx1
+        (DIV: diverge_index _ idx1 (ktr x))
+        (IDX: forall i, idx1 i <= idx0 i)
+      :
+      _diverge_index diverge_index idx0 (Vis (Choose X) ktr)
+    | diverge_index_fair
+        m ktr idx0 idx1
+        (DIV: diverge_index _ idx1 (ktr tt))
+        (EMP: forall j (IDX: (m j) = Flag.emp), idx1 j <= idx0 j)
+        (FAIL: forall j (IDX: (m j) = Flag.fail), idx1 j < idx0 j)
+      :
+      _diverge_index diverge_index idx0 (Vis (Fair m) ktr)
+    | diverge_index_syscall
+        fn args retv ktr idx0 idx1
+        (DIV: diverge_index _ idx1 (ktr retv))
+        (IDX: forall i, idx1 i <= idx0 i)
+      :
+      _diverge_index diverge_index idx0 (Vis (Syscall fn args retv) ktr)
   .
 
   Lemma diverge_index_mon: monotone3 _diverge_index.
@@ -120,11 +163,469 @@ Section BEHAVES.
     - econs 1; eauto.
     - econs 2; eauto.
     - econs 3; eauto.
+    - econs 4; eauto.
   Qed.
 
-  Definition diverge_index: forall (R: Type) (idx: Ident.(id) -> nat) (itr: itree eventE R), Prop := paco3 _diverge_index bot3.
+  Definition diverge_index: forall (R: Type) (idx: id -> nat) (itr: itree eventE R), Prop := paco3 _diverge_index bot3.
 
   Definition diverge (R: Type) (itr: itree eventE R): Prop :=
     exists idx, diverge_index idx itr.
 
 End BEHAVES.
+
+
+
+Section STS.
+
+  Context {Ident: ID}.
+
+  Definition state {R} := itree eventE R.
+
+  Inductive step {R}: @state R -> option event -> state -> Prop :=
+  | step_tau
+      itr
+    :
+    step (Tau itr) None itr
+  | step_choose
+      X ktr (x: X)
+    :
+    step (Vis (Choose X) ktr) None (ktr x)
+  | step_fair
+      m ktr
+    :
+    step (Vis (Fair m) ktr) None (ktr tt)
+  | step_syscall
+      fn args retv ktr
+    :
+    step (Vis (Syscall fn args retv) ktr) (Some (event_syscall fn args retv)) (ktr retv)
+  .
+
+  Lemma step_trigger_choose_iff X k itr e
+        (STEP: step (trigger (Choose X) >>= k) e itr)
+    :
+      exists x,
+        e = None /\ itr = k x.
+  Proof.
+    inv STEP.
+    { eapply f_equal with (f:=observe) in H0. ss. }
+    { eapply f_equal with (f:=observe) in H0. ss.
+      unfold trigger in H0. ss. cbn in H0.
+      dependent destruction H0. ired. et.  }
+    { eapply f_equal with (f:=observe) in H0. ss. }
+    { eapply f_equal with (f:=observe) in H0. ss. }
+  Qed.
+
+  Lemma step_trigger_take_iff X k itr e
+        (STEP: step (trigger (Take X) >>= k) e itr)
+    :
+      exists x,
+        e = None /\ itr = k x.
+  Proof.
+    inv STEP.
+    { eapply f_equal with (f:=observe) in H0. ss. }
+    { eapply f_equal with (f:=observe) in H0. ss. }
+    { eapply f_equal with (f:=observe) in H0. ss.
+      unfold trigger in H0. ss. cbn in H0.
+      dependent destruction H0. ired. et.  }
+    { eapply f_equal with (f:=observe) in H0. ss. }
+  Qed.
+
+  Lemma step_tau_iff itr0 itr1 e
+        (STEP: step (Tau itr0) e itr1)
+    :
+      e = None /\ itr0 = itr1.
+  Proof.
+    inv STEP. et.
+  Qed.
+
+  Lemma step_ret_iff rv itr e
+        (STEP: step (Ret rv) e itr)
+    :
+      False.
+  Proof.
+    inv STEP.
+  Qed.
+
+  Lemma step_trigger_syscall_iff fn args rvs k e itr
+        (STEP: step (trigger (Syscall fn args rvs) >>= k) e itr)
+    :
+      exists rv, itr = k rv /\ e = Some (event_sys fn args rv)
+                 /\ <<RV: rvs rv>> /\ <<SYS: syscall_sem (event_sys fn args rv)>>.
+  Proof.
+    inv STEP.
+    { eapply f_equal with (f:=observe) in H0. ss. }
+    { eapply f_equal with (f:=observe) in H0. ss. }
+    { eapply f_equal with (f:=observe) in H0. ss. }
+    { eapply f_equal with (f:=observe) in H0. ss.
+      unfold trigger in H0. ss. cbn in H0.
+      dependent destruction H0. ired. et. }
+  Qed.
+
+
+  Let itree_eta E R (itr0 itr1: itree E R)
+      (OBSERVE: observe itr0 = observe itr1)
+    :
+      itr0 = itr1.
+  Proof.
+    rewrite (itree_eta_ itr0).
+    rewrite (itree_eta_ itr1).
+    rewrite OBSERVE. auto.
+  Qed.
+
+  Lemma step_trigger_choose X k x
+    :
+      step (trigger (Choose X) >>= k) None (k x).
+  Proof.
+    unfold trigger. ss.
+    match goal with
+    | [ |- step ?itr _ _] =>
+      replace itr with (Subevent.vis (Choose X) k)
+    end; ss.
+    { econs. }
+    { eapply itree_eta. ss. cbv. f_equal.
+      extensionality x0. eapply itree_eta. ss. }
+  Qed.
+
+  Lemma step_trigger_take X k x
+    :
+      step (trigger (Take X) >>= k) None (k x).
+  Proof.
+    unfold trigger. ss.
+    match goal with
+    | [ |- step ?itr _ _] =>
+      replace itr with (Subevent.vis (Take X) k)
+    end; ss.
+    { econs. }
+    { eapply itree_eta. ss. cbv. f_equal.
+      extensionality x0. eapply itree_eta. ss. }
+  Qed.
+
+  Lemma step_trigger_syscall fn args (rvs: Any.t -> Prop) k rv
+        (RV: rvs rv) (SYS: syscall_sem (event_sys fn args rv))
+    :
+      step (trigger (Syscall fn args rvs) >>= k) (Some (event_sys fn args rv)) (k rv).
+  Proof.
+    unfold trigger. ss.
+    match goal with
+    | [ |- step ?itr _ _] =>
+      replace itr with (Subevent.vis (Syscall fn args rvs) k)
+    end; ss.
+    { econs; et. }
+    { eapply itree_eta. ss. cbv. f_equal.
+      extensionality x0. eapply itree_eta. ss. }
+  Qed.
+
+
+End STS.
+
+
+
+
+Module Beh.
+
+Definition t: Type := Tr.t -> Prop.
+Definition improves (src tgt: t): Prop := tgt <1= src.
+
+Section BEHAVES.
+
+  Definition union (st0: state) (P: (option event) -> state -> Prop) :=
+    exists ev st1, (<<STEP: L.(step) st0 ev st1>>) /\ (<<UNION: P ev st1>>).
+  (* Definition inter (st0: L.(state)) (P: (option event) -> L.(state) -> Prop) := *)
+  (*   forall ev st1 (STEP: L.(step) st0 ev st1), <<INTER: P ev st1>>. *)
+
+  Inductive _state_spin (state_spin: L.(state) -> Prop)
+            (st0: L.(state)): Prop :=
+  | state_spin_angelic
+      (SRT: L.(state_sort) st0 = angelic)
+      (STEP: forall ev st1 (STEP: L.(step) st0 ev st1), <<TL: state_spin st1>>)
+  | state_spin_demonic
+      (SRT: L.(state_sort) st0 = demonic)
+      (STEP: exists ev st1 (STEP: L.(step) st0 ev st1), <<TL: state_spin st1>>)
+  .
+
+  Definition state_spin: _ -> Prop := paco1 _state_spin bot1.
+
+  Lemma state_spin_mon: monotone1 _state_spin.
+  Proof.
+    ii. inv IN; try (by econs; eauto).
+    - econs 1; et. ii. exploit STEP; et.
+    - des. econs 2; et. esplits; et.
+  Qed.
+
+  Hint Constructors _state_spin.
+  Hint Unfold state_spin.
+  Hint Resolve state_spin_mon: paco.
+
+
+
+  Inductive _of_state (of_state: L.(state) -> Tr.t -> Prop): L.(state) -> Tr.t -> Prop :=
+  | sb_final
+      st0 retv
+      (FINAL: L.(state_sort) st0 = final retv)
+    :
+    _of_state of_state st0 (Tr.done retv)
+  | sb_spin
+      st0
+      (SPIN: state_spin st0)
+    :
+    _of_state of_state st0 (Tr.spin)
+  | sb_nb
+      st0
+    :
+    _of_state of_state st0 (Tr.nb)
+  | sb_vis
+      st0 st1 ev evs
+      (SRT: L.(state_sort) st0 = vis)
+      (STEP: _.(step) st0 (Some ev) st1)
+      (TL: of_state st1 evs)
+    :
+    _of_state of_state st0 (Tr.cons ev evs)
+  | sb_demonic
+      st0
+      evs
+      (SRT: L.(state_sort) st0 = demonic)
+      (STEP: union st0 (fun e st1 => (<<HD: e = None>>) /\ (<<TL: _of_state of_state st1 evs>>)))
+    :
+    _of_state of_state st0 evs
+  | sb_angelic
+      st0
+      evs
+      (SRT: L.(state_sort) st0 = angelic)
+      (STEP: inter st0 (fun e st1 => (<<HD: e = None>>) /\ (<<TL: _of_state of_state st1 evs>>)))
+    :
+    _of_state of_state st0 evs
+  .
+
+  Definition of_state: _ -> _ -> Prop := paco2 _of_state bot2.
+
+  Theorem of_state_ind :
+    forall (r P: _ -> _ -> Prop),
+      (forall st0 retv, state_sort L st0 = final retv -> P st0 (Tr.done retv)) ->
+      (forall st0, state_spin st0 -> P st0 Tr.spin) ->
+      (forall st0, P st0 Tr.nb) ->
+
+      (forall st0 st1 ev evs
+         (SRT: state_sort L st0 = vis)
+         (STEP: _.(step) st0 (Some ev) st1)
+         (TL: r st1 evs)
+        ,
+          P st0 (Tr.cons ev evs)) ->
+      (forall st0 evs
+         (SRT: state_sort L st0 = demonic)
+         (STEP: union st0
+                      (fun e st1 =>
+                         <<HD: e = None >> /\ <<TL: _of_state r st1 evs >> /\ <<IH: P st1 evs>>)), P st0 evs) ->
+      (forall st0 evs
+         (* (IH: forall st1 (STEP: L.(step) st0 None st1), P st1 evs) *)
+         (SRT: state_sort L st0 = angelic)
+         (STEP: inter st0
+                      (fun e st1 => <<HD: e = None >> /\ <<TL: _of_state r st1 evs >> /\ <<IH: P st1 evs>>)),
+          P st0 evs) ->
+      forall s t, _of_state r s t -> P s t.
+  Proof.
+    (* fix IH 11. i. *)
+    (* inv H5; eauto. *)
+    (* - eapply H3; eauto. rr in STEP. des; clarify. *)
+    (*   + esplits; eauto. rr. esplits; eauto. left. esplits; eauto. eapply IH; eauto. Guarded. *)
+    (*   + esplits; eauto. rr. esplits; eauto. right. esplits; eauto. *)
+    (* - eapply H4; eauto. ii. exploit STEP; eauto. i; des; clarify. *)
+    (*   + esplits; eauto. left. esplits; eauto. eapply IH; eauto. *)
+    (*   + esplits; eauto. right. esplits; eauto. *)
+    fix IH 11. i.
+    inv H5; eauto.
+    - eapply H3; eauto. rr in STEP. des; clarify. esplits; eauto. rr. esplits; eauto. eapply IH; eauto.
+    - eapply H4; eauto. ii. exploit STEP; eauto. i; des; clarify. esplits; eauto. eapply IH; eauto.
+  Qed.
+
+  Lemma of_state_mon: monotone2 _of_state.
+  Proof.
+    ii. induction IN using of_state_ind; eauto.
+    - econs 1; et.
+    - econs 2; et.
+    - econs 3; et.
+    - econs 4; et.
+    - econs 5; et. rr in STEP. des; clarify. rr. esplits; et.
+    - econs 6; et. ii. exploit STEP; eauto. i; des; clarify.
+  Qed.
+
+  Hint Constructors _of_state.
+  Hint Unfold of_state.
+  Hint Resolve of_state_mon: paco.
+
+  Definition of_program: Tr.t -> Prop := of_state L.(initial_state).
+
+
+
+
+  (**********************************************************)
+  (*********************** properties ***********************)
+  (**********************************************************)
+
+  Lemma prefix_closed_state
+        st0 pre bh
+        (BEH: of_state st0 bh)
+        (PRE: Tr.prefix pre bh)
+    :
+    <<NB: of_state st0 (Tr.app pre Tr.nb)>>
+  .
+  Proof.
+    revert_until L. pcofix CIH. i. punfold BEH. rr in PRE. des; subst.
+    destruct pre; ss; clarify.
+    { pfold. econs; eauto. }
+
+    remember (Tr.cons e (Tr.app pre tl)) as tmp. revert Heqtmp.
+    induction BEH using of_state_ind; ii; ss; clarify.
+    - pclearbot. pfold. econs; eauto. right. eapply CIH; et. rr; et.
+    - pfold. econs 5; eauto. rr in STEP. des; clarify. rr. esplits; eauto.
+      exploit IH; et. intro A. punfold A.
+    - pfold. econs 6; eauto. ii. exploit STEP; eauto. clear STEP. i; des; clarify. esplits; eauto.
+      exploit IH; et. intro A. punfold A.
+  Qed.
+
+  Theorem prefix_closed
+          pre bh
+          (BEH: of_program bh)
+          (PRE: Tr.prefix pre bh)
+    :
+    <<NB: of_program (Tr.app pre Tr.nb)>>
+  .
+  Proof.
+    eapply prefix_closed_state; eauto.
+  Qed.
+
+  Lemma nb_bottom
+        st0
+    :
+    <<NB: of_state st0 Tr.nb>>
+  .
+  Proof. pfold. econs; et. Qed.
+
+  Lemma ub_top
+        st0
+        (UB: of_state st0 Tr.ub)
+    :
+    forall beh, of_state st0 beh
+  .
+  Proof.
+    revert_until L. pfold. i. punfold UB.
+    remember Tr.ub as tmp. revert Heqtmp.
+    induction UB using of_state_ind; ii; ss; clarify.
+    - rr in STEP. des. clarify. econs; eauto. rr. esplits; eauto.
+    - econs 6; eauto. ii. exploit STEP; eauto. i; des; clarify. esplits; eauto.
+  Qed.
+
+  Lemma _beh_astep
+        r tr st0 ev st1
+        (SRT: L.(state_sort) st0 = angelic)
+        (STEP: _.(step) st0 ev st1)
+        (BEH: paco2 _of_state r st0 tr)
+    :
+    <<BEH: paco2 _of_state r st1 tr>>
+  .
+  Proof.
+    exploit wf_angelic; et. i; clarify.
+    revert_until L.
+    pcofix CIH; i.
+    punfold BEH.
+    {
+      generalize dependent st1.
+      induction BEH using of_state_ind; et; try rewrite SRT in *; ii; ss.
+      - punfold H. inv H; rewrite SRT in *; ss.
+        exploit STEP0; et. i; des. pclearbot. et.
+      - rr in STEP. exploit STEP; et. i; des.
+        pfold. eapply of_state_mon; et. ii; ss. eapply upaco2_mon; et.
+    }
+  Qed.
+
+  Lemma beh_astep
+        tr st0 ev st1
+        (SRT: L.(state_sort) st0 = angelic)
+        (STEP: _.(step) st0 ev st1)
+        (BEH: of_state st0 tr)
+    :
+    <<BEH: of_state st1 tr>>
+  .
+  Proof.
+    eapply _beh_astep; et.
+  Qed.
+
+  Lemma _beh_dstep
+        r tr st0 ev st1
+        (SRT: L.(state_sort) st0 = demonic)
+        (STEP: _.(step) st0 ev st1)
+        (BEH: paco2 _of_state r st1 tr)
+    :
+    <<BEH: paco2 _of_state r st0 tr>>
+  .
+  Proof.
+    exploit wf_demonic; et. i; clarify.
+    pfold. econs 5; et. rr. esplits; et. punfold BEH.
+  Qed.
+
+  Lemma beh_dstep
+        tr st0 ev st1
+        (SRT: L.(state_sort) st0 = demonic)
+        (STEP: _.(step) st0 ev st1)
+        (BEH: of_state st1 tr)
+    :
+    <<BEH: of_state st0 tr>>
+  .
+  Proof.
+    eapply _beh_dstep; et.
+  Qed.
+
+  Variant dstep_clo (r: L.(state) -> Tr.t -> Prop): L.(state) -> Tr.t -> Prop :=
+    | dstep_clo_intro
+        st0 tr st1 ev
+        (SRT: L.(state_sort) st0 = demonic)
+        (STEP: _.(step) st0 ev st1)
+        (STEP: r st1 tr)
+      :
+      dstep_clo r st0 tr
+  .
+
+  Lemma dstep_clo_mon: monotone2 dstep_clo.
+  Proof. ii. inv IN. econs; et. Qed.
+
+  Lemma dstep_clo_spec: dstep_clo <3= gupaco2 (_of_state) (cpn2 _of_state).
+  Proof.
+    intros. eapply prespect2_uclo; eauto with paco. econs.
+    { eapply dstep_clo_mon. }
+    i. inv PR0. pfold. econs 5; et.
+    exploit wf_demonic; et. i; clarify.
+    red. esplits; et. eapply of_state_mon; et.
+  Qed.
+
+  Variant astep_clo (r: L.(state) -> Tr.t -> Prop): L.(state) -> Tr.t -> Prop :=
+    | astep_clo_intro
+        st0 tr
+        (SRT: L.(state_sort) st0 = angelic)
+        (STEP: forall st1, _.(step) st0 None st1 -> r st1 tr)
+      :
+      astep_clo r st0 tr
+  .
+
+  Lemma astep_clo_mon: monotone2 astep_clo.
+  Proof. ii. inv IN. econs; et. Qed.
+
+  Lemma astep_clo_spec: astep_clo <3= gupaco2 (_of_state) (cpn2 _of_state).
+  Proof.
+    intros. eapply prespect2_uclo; eauto with paco. econs.
+    { eapply astep_clo_mon. }
+    i. inv PR0. pfold. econs 6; et. ii.
+    exploit wf_angelic; et. i; clarify.
+    red. esplits; et. eapply of_state_mon; et.
+  Qed.
+
+End BEHAVES.
+
+End Beh.
+Hint Unfold Beh.improves.
+Hint Constructors Beh._state_spin.
+Hint Unfold Beh.state_spin.
+Hint Resolve Beh.state_spin_mon: paco.
+Hint Constructors Beh._of_state.
+Hint Unfold Beh.of_state.
+Hint Resolve Beh.of_state_mon: paco.
+
+
